TvmLean/Model/Cont/Cdata.lean
@@ -1,1 +1,7 @@
-import TvmLean.Model.Internal
+import TvmLean.Model.Cont.Cregs
+
+namespace TvmLean
+
+def OrdCdata.empty : OrdCdata := {}
+
+end TvmLean
