TvmLean/Model/Error/Excno.lean
@@ -1,1 +1,60 @@
-import TvmLean.Model.Internal
+import Std
+
+namespace TvmLean
+
+inductive Excno : Type
+  | none
+  | alt
+  | stkUnd
+  | stkOv
+  | intOv
+  | rangeChk
+  | invOpcode
+  | typeChk
+  | cellOv
+  | cellUnd
+  | dictErr
+  | unknown
+  | unimplemented
+  | fatal
+  | outOfGas
+  | virtErr
+  deriving DecidableEq, Repr, Inhabited
+
+def Excno.toInt : Excno → Int
+  | .none => 0
+  | .alt => 1
+  | .stkUnd => 2
+  | .stkOv => 3
+  | .intOv => 4
+  | .rangeChk => 5
+  | .invOpcode => 6
+  | .typeChk => 7
+  | .cellOv => 8
+  | .cellUnd => 9
+  | .dictErr => 10
+  | .unknown => 11
+  | .fatal => 12
+  | .outOfGas => 13
+  | .virtErr => 14
+  | .unimplemented => 15
+
+instance : ToString Excno := ⟨fun
+  | .none => "none"
+  | .alt => "alt"
+  | .stkUnd => "stkUnd"
+  | .stkOv => "stkOv"
+  | .intOv => "intOv"
+  | .rangeChk => "rangeChk"
+  | .invOpcode => "invOpcode"
+  | .typeChk => "typeChk"
+  | .cellOv => "cellOv"
+  | .cellUnd => "cellUnd"
+  | .dictErr => "dictErr"
+  | .unknown => "unknown"
+  | .unimplemented => "unimplemented"
+  | .fatal => "fatal"
+  | .outOfGas => "outOfGas"
+  | .virtErr => "virtErr"⟩
+
+end TvmLean
