TvmLean/Model/Stack/Stack.lean
@@ -1,1 +1,7 @@
-import TvmLean.Model.Internal
+import TvmLean.Model.Value.Value
+
+namespace TvmLean
+
+abbrev Stack := Array Value
+
+end TvmLean
