TvmLean/Model/State/Registers.lean
@@ -1,1 +1,24 @@
-import TvmLean.Model.Internal
+import TvmLean.Model.Instr.Asm.Cp0
+
+namespace TvmLean
+
+structure Regs where
+  c0 : Continuation
+  c1 : Continuation
+  c2 : Continuation
+  c3 : Continuation
+  c4 : Cell
+  c5 : Cell
+  c7 : Array Value
+  deriving Repr
+
+def Regs.initial : Regs :=
+  { c0 := .quit 0
+    c1 := .quit 1
+    c2 := .excQuit
+    c3 := .quit 11
+    c4 := Cell.empty
+    c5 := Cell.empty
+    c7 := #[] }
+
+end TvmLean
