TvmLean/Model/Value/Value.lean
@@ -1,1 +1,59 @@
-import TvmLean.Model.Internal
+import TvmLean.Model.Cont.Continuation
+
+namespace TvmLean
+
+instance : Inhabited Value := ⟨.null⟩
+
+def Value.pretty : Value → String
+  | .int .nan => "NaN"
+  | .int (.num n) => toString n
+  | .null => "null"
+  | .cell _ => "<cell>"
+  | .slice _ => "<slice>"
+  | .builder _ => "<builder>"
+  | .tuple t => s!"<tuple:{t.size}>"
+  | .cont k =>
+      match k with
+      | .ordinary _ _ _ _ => "<cont:ord>"
+      | .envelope _ _ _ => "<cont:env>"
+      | .quit n => s!"<cont:quit {n}>"
+      | .excQuit => "<cont:excquit>"
+      | .whileCond _ _ _ => "<cont:while-cond>"
+      | .whileBody _ _ _ => "<cont:while-body>"
+      | .untilBody _ _ => "<cont:until-body>"
+      | .repeatBody _ _ _ => "<cont:repeat-body>"
+      | .againBody _ => "<cont:again-body>"
+
+instance : ToString Value := ⟨Value.pretty⟩
+
+def arrayBeqBy {α : Type} (a b : Array α) (beq : α → α → Bool) : Bool :=
+  if a.size != b.size then
+    false
+  else
+    Id.run do
+      let mut ok := true
+      for i in [0:a.size] do
+        match a.get? i, b.get? i with
+        | some x, some y =>
+            if !(beq x y) then
+              ok := false
+        | _, _ =>
+            ok := false
+      return ok
+
+def arrayBeq {α : Type} [BEq α] (a b : Array α) : Bool :=
+  arrayBeqBy a b (fun x y => x == y)
+
+partial def Value.beq : Value → Value → Bool
+  | .null, .null => true
+  | .int x, .int y => x == y
+  | .cell x, .cell y => x == y
+  | .slice x, .slice y => x == y
+  | .builder x, .builder y => x == y
+  | .tuple x, .tuple y => arrayBeqBy x y Value.beq
+  | .cont x, .cont y => x == y
+  | _, _ => false
+
+instance : BEq Value := ⟨Value.beq⟩
+
+end TvmLean
