TvmLean/Semantics/VM/Monad.lean
@@ -1,1 +1,7 @@
-import TvmLean.Model
+import TvmLean.Model.State.VmState
+
+namespace TvmLean
+
+abbrev VM := ExceptT Excno (StateM VmState)
+
+end TvmLean
